cfrontend/BeePL_operators_proofs.v
@@ -1,0 +1,48 @@
+Require Import String ZArith Coq.FSets.FMapAVL Coq.Structures.OrderedTypeEx FunInd.
+Require Import Coq.FSets.FSetProperties Coq.FSets.FMapFacts FMaps FSetAVL Nat PeanoNat Linking.
+Require Import Coq.Arith.EqNat Coq.ZArith.Int Integers AST Maps Linking Ctypes Smallstep SimplExpr.
+Require Import compcert.common.Errors Initializersproof Cstrategy BeePL_auxlemmas Coqlib Errors Memory.
+Require Import BeePL_aux BeePL_mem BeeTypes BeePL Csyntax Clight Globalenvs BeePL_Csyntax SimplExpr.
+Require Import BeePL_sem BeePL_typesystem BeePL_compiler_proofs BeePL_values BeePL_notations.
+
+From mathcomp Require Import all_ssreflect.
+
+(* notbool are well-formed *) 
+Lemma well_formed_notbool : forall cenv Gamma Sigma bge vm m v ef,
+store_well_typed cenv Gamma Sigma bge vm m ->
+type_expr cenv Gamma Sigma (Val v (Vtype Tbool)) ef (Vtype Tbool) ->
+exists v' v'',
+Cop.sem_unary_operation (Cop.Onotbool) (trans_bvalue_cvalue v) (transBeePL_type (Vtype Tbool)) m = Some v' /\
+v' <> Values.Vundef /\
+trans_cvalue_bvalue v' = OK v''.
+Proof.
+move=> cenv Gamma Sigma bge vm m v ef hw hte. 
+rewrite / Cop.sem_unary_operation /= /Cop.sem_notbool /= /option_map /=.
+case: v hte=> //=.
+(* unit : bad case *)
++ move=> hte. by inversion hte.
+(* bool : good case *)
++ move=> b hte. case: b hte=> //=. 
+  (* b = true *)
+  + move=> hte. rewrite /Values.Val.of_bool /=.
+    have hn : ~~ ~~ Int.eq (Int.repr 1) Int.zero = false.
+    + rewrite /negb /=. have hz : Int.eq (Int.repr 1) Int.zero = false.
+      + by auto. by rewrite hz /=.
+    rewrite hn /=. exists Values.Vfalse. rewrite /trans_cvalue_bvalue /=. 
+    by exists (Vint Int.zero).
+  (* b = false *)
+  move=> hte. rewrite /Values.Val.of_bool /=.
+  have hn : ~~ ~~ Int.eq (Int.repr 0) Int.zero = true.
+  + rewrite /negb /=. have hz : Int.eq (Int.repr 0) Int.zero = true.
+    + by auto. by rewrite hz /=.
+  rewrite hn /=. exists Values.Vtrue. rewrite /trans_cvalue_bvalue /=. 
+  by exists (Vint Int.one).
+(* int : bad case *)
++ move=> i hte. by inversion hte.
+(* int64 : bad case *)
++ move=> l hte. by inversion hte.
+(* ptr : bad case *)
++ move=> p o hte. by inversion hte.
+(* o : bad case *)
+move=> o hte. by inversion hte.
+Qed.
