cfrontend/BeePL_typechecker.v
@@ -94,7 +94,7 @@ match e with
                                                   | Ptrtype pt => do (te2, ef2) <- type_check_expr cenv Gamma Sigma e2;
                                                                   let bt := get_data_type pt in
                                                                   match te2 with 
-                                                                  | bt => if eq_type t Utype
+                                                                  | bt => if eq_type t Utype && (is_option_ptr_type pt == false) 
                                                                                 then OK (Utype, ef1 ++ ef2 ++ (Write mem_ident :: nil))
                                                                                 else Error (msg "Massgntype does not match the inferred type")
                                                                                       end 
